---
title: "Exercise 7.3"
subtitle: "Special Cases of the CES Armington Aggregator"
---
<a class="return-button" href="index.qmd">â¬… Return</a>

## Problem

Consider the  CES Armington aggregator 

$$
A(a^m,a^x) = 
\left[
\chi 
\left(a^m\right)^{1-\frac1{\mu}}
+ (1-\chi)
\left(a^x\right)^{1-\frac1{\mu}}
\right]^{\frac{1}{1-\frac{1}{\mu}}}.
$$

Show that 

$$
\lim_{\mu\rightarrow1}A(a^m,a^x)= (a^m)^{\chi}(a^x)^{1-\chi}.
$$

$$
\lim_{\mu\rightarrow0}A(a^m,a^x)= 
\min\{ a^m,a^x\}. 
$$

and

$$
\lim_{\mu\rightarrow\infty}A(a^m,a^x)= 
\chi a^m + (1-\chi)a^x.
$$

Note that the share parameter $\chi$ drops from the Armington aggregator as $\mu\rightarrow 0$. This may be an undesirable property for  certain applications. Provide an alternative specification of the CES aggregator such that 

$$
\lim_{\mu\rightarrow0}A(a^m,a^x)= 
\min\{ \chi a^m,(1-\chi)a^x\}.
$$

## Answer

We first show that

Use

$$ 
\ln A(a^m,a^x) = \frac{\ln \left[
\chi 
\left(a^m\right)^{1-\frac1{\mu}}
+ (1-\chi)
\left(a^x\right)^{1-\frac1{\mu}}
\right]}{1-\frac{1}{\mu}}
$$

For $\mu=1$ this is not defined because the denominator is $0$. Thus let's apply the  l'Hospital rule.

$$
\begin{eqnarray*}
&\lim_{\mu\rightarrow 1} \frac{\ln \left[
\chi 
\left(a^m\right)^{1-\frac1{\mu}}
+ (1-\chi)
\left(a^x\right)^{1-\frac1{\mu}}
\right]}{1-\frac{1}{\mu}} 
 \\
=&\lim_{\mu\rightarrow 1} 
\frac{\frac1{ \left[
\chi 
\left(a^m\right)^{1-\frac1{\mu}}
+ (1-\chi)
\left(a^x\right)^{1-\frac1{\mu}}
\right]} \left[\chi \ln a^m \frac1{\mu^2} \left(a^m\right)^{1-\frac1{\mu}}
+ (1-\chi) \ln a^x \frac1{\mu^2} \left(a^x\right)^{1-\frac1{\mu}}\right]}{\frac{1}{\mu^2}}\\
=&\chi \ln a^m + (1-\chi) \ln a^x 
\\
=&\ln\left[ \left(a^m\right)^{\chi}\left(a^x\right)^{(1-\chi)} \right]
\end{eqnarray*}
$$

Next, we show that

Note that 

$$
\lim_{\mu\rightarrow 0} \frac{1}{1-\frac{1}{\mu}} = 
\lim_{\mu\rightarrow 0} \frac{\mu}{\mu -1} =  \frac{0}{-1} =0
$$

and that 

$$
\lim_{\mu\rightarrow 0} \left(1-\frac{1}{\mu}\right) = -\infty
$$

Suppose that $a^m/a^x>1$, so that $(a^m/a^x)^{-\infty} =0$
Take out $a^x$

$$
A(a^m,a^x) = a^x
\left[
\chi  \left(a^m/a^x
\right)^{1-\frac1{\mu}}
+ (1-\chi)
\right]^\frac1{{1-\frac{1}{\mu}}}
$$

Now the part in the square brackets is well defined as $\mu\rightarrow 0$ so that 

$$
\lim_{\mu\rightarrow 0} \left[
\chi  \left(a^m/a^x
\right)^{1-\frac1{\mu}}
+ (1-\chi)
\right]^\frac1{{1-\frac{1}{\mu}}}
= \left[
 (1-\chi)
\right]^0
= 1
$$

and hence if $a^m/a^x>1$, then  

$$
\lim_{\mu \rightarrow 0} A(a^m,a^x) = a^x
$$

By the same argument we have that if if $a^m/a^x<1$, then  

$$
\lim_{\mu \rightarrow 0} A(a^m,a^x) = a^m
$$

It follows that 

$$
\lim_{\mu \rightarrow 0} A(a^m,a^x) = \min\{a^m, a^x\}, 
$$

which is what we were asked to show. 

Then, we show that

The claim follows from the facts that 

$$
\lim_{\mu\rightarrow \infty} \frac{1}{1-\frac{1}{\mu}} = 1
$$

and 

$$
\lim_{\mu\rightarrow \infty} \left(1-\frac{1}{\mu}\right) = 1.
$$

Finally, we propose an alternative specification such that

Let 

$$
A(a^m,a^x) = 
\left[
\left(
\chi  a^m 
\right)^{1-\frac1{\mu}}
+ \left(
(1-\chi)  a^x \right)^{1-\frac1{\mu}}
\right]
^\frac1{{1-\frac{1}{\mu}}}
$$

Suppose $\chi a^m<(1-\chi) a^x$, then we have: 

$$
A(a^m,a^x) =  \chi a^m
\left[
1 
+ 
\left(\frac{
(1-\chi)  a^x 
}
{\chi a^m}
\right)^{1-\frac1{\mu}}
\right]
^\frac1{{1-\frac{1}{\mu}}}
$$

For the rest proceed as above.